cleanq/crb: reorganize a few lemmas
Signed-off-by: Reto Achermann <reto.achermann@inf.ethz.ch>

CleanQ/CleanQ_CRBModel.thy
@@ -164,341 +164,7 @@ lemma frame_rb_weak_y_list_weak:
 
 
 
-(* ==================================================================================== *)
-subsection \<open>State Transition Operations\<close>
-(* ==================================================================================== *)
 
-text \<open>
-  We now formulate the state transition operations in terms of the CleanQ RB model
-  state. Again, the two agents can, independently from each other, perform one of 
-  two operations, \verb+enqueue+ and \verb+dequeue+,  which trigger an ownership 
-  transfer of buffer elements. In the previous model we implemented \verb+enqueue+ and
-  \verb+dequeue+ as a single atomic step. Here we define it as two steps each.   
-
-  We will first show that the enqueue and dequeue operations in two calls are
-  the same as the atomic step and also preserve the invariant. This is basically
-  showing equivalence in the non concurrent setting
-\<close>
-
-(* ------------------------------------------------------------------------------------ *)
-subsubsection \<open>Enqueue Operation\<close>
-(* ------------------------------------------------------------------------------------ *)
-
-text \<open>
-  The first part of the \verb+enqueue+ operation is to write head buffer element into
-  the ring at the head position.
-\<close>
-
-definition CleanQ_RB_write_head_x :: "'a \<Rightarrow> 'a CleanQ_RB_State \<Rightarrow> 'a CleanQ_RB_State" 
-  where "CleanQ_RB_write_head_x b rb = rb \<lparr>rTXY := rb_write_head b (rTXY rb) \<rparr>"
-
-definition CleanQ_RB_write_head_y :: "'a \<Rightarrow> 'a CleanQ_RB_State \<Rightarrow> 'a CleanQ_RB_State" 
-  where "CleanQ_RB_write_head_y b rb = rb \<lparr>rTYX := rb_write_head b (rTYX rb) \<rparr>"
-
-text \<open>
-  The second part is to increment the head pointer, this effectively transfers the 
-  ownership of the buffer from the owning sets SX or SY to the transfer set TXY or TYX. 
-\<close>
-
-definition CleanQ_RB_incr_head_x :: "'a \<Rightarrow> 'a CleanQ_RB_State \<Rightarrow> 'a CleanQ_RB_State" 
-  where "CleanQ_RB_incr_head_x b rb = rb \<lparr>rTXY := rb_incr_head (rTXY rb), 
-                                          rSX := (rSX rb) - {b} \<rparr>"
-
-definition CleanQ_RB_incr_head_y :: "'a \<Rightarrow> 'a CleanQ_RB_State \<Rightarrow> 'a CleanQ_RB_State" 
-  where "CleanQ_RB_incr_head_y b rb = rb \<lparr> rTYX := rb_incr_head (rTYX rb), 
-                                           rSY := (rSY rb) - {b} \<rparr>"
-
-
-text \<open>
-  We define helper functions to read the head pointer of the ring buffer and to check
-  whether the head position of the ring is \verb+None+ or it contains some buffer.
-\<close>
-
-definition CleanQ_RB_read_head_x :: "'a CleanQ_RB_State \<Rightarrow> 'a " 
-  where "CleanQ_RB_read_head_x rb = rb_read_head (rTXY rb)"
-
-definition CleanQ_RB_read_head_y :: "'a CleanQ_RB_State \<Rightarrow> 'a " 
-  where "CleanQ_RB_read_head_y rb = rb_read_head (rTYX rb)"
-
-definition CleanQ_RB_head_none_x :: "'a CleanQ_RB_State \<Rightarrow> bool" 
-  where "CleanQ_RB_head_none_x rb = rb_head_none (rTXY rb)"
-
-definition CleanQ_RB_head_none_y :: "'a CleanQ_RB_State \<Rightarrow> bool" 
-  where "CleanQ_RB_head_none_y rb = rb_head_none (rTYX rb)"
-
-
-text \<open> 
-  Writing the head location in the ring ensures that the head is not none. 
-\<close>
-
-lemma CleanQ_RB_head_write_x_not_none:
-  "\<not>CleanQ_RB_head_none_x (CleanQ_RB_write_head_x b rb)"
-  unfolding CleanQ_RB_head_none_x_def CleanQ_RB_write_head_x_def
-  by (simp add: rb_write_head_not_none)
-
-lemma CleanQ_RB_head_write_y_not_none:
-  "\<not>CleanQ_RB_head_none_y (CleanQ_RB_write_head_y b rb)"
-  unfolding CleanQ_RB_head_none_y_def CleanQ_RB_write_head_y_def
-  by (simp add: rb_write_head_not_none)
-
-lemma CleanQ_RB_write_head_read_head_x:
-  "b = CleanQ_RB_read_head_x (CleanQ_RB_write_head_x b rb)"
-  unfolding CleanQ_RB_read_head_x_def CleanQ_RB_write_head_x_def
-  by (simp add: rb_read_head_def rb_write_head_element_read)
-
-lemma CleanQ_RB_write_head_read_head_y:
-  "b = CleanQ_RB_read_head_y (CleanQ_RB_write_head_y b rb)"
-  unfolding CleanQ_RB_read_head_y_def CleanQ_RB_write_head_y_def
-  by (simp add: rb_read_head_def rb_write_head_element_read)
-
-
-text \<open>
-  We first show, that the combination of the two operation, yields the original 
-  \verb+enqueue+ operation of the sequential ring buffer model. We add those two to
-  the simp set.
-\<close>
-
-lemma CleanQ_RB_enq_x_split_equal[simp]:
-  "CleanQ_RB_incr_head_x b (CleanQ_RB_write_head_x b rb) = CleanQ_RB_enq_x b rb"
-  unfolding CleanQ_RB_incr_head_x_def CleanQ_RB_write_head_x_def CleanQ_RB_enq_x_def
-  rb_enq_def by simp
-
-lemma CleanQ_RB_enq_y_split_equal[simp]:
-  "CleanQ_RB_incr_head_y b (CleanQ_RB_write_head_y b rb) = CleanQ_RB_enq_y b rb"
-  unfolding CleanQ_RB_incr_head_y_def CleanQ_RB_write_head_y_def CleanQ_RB_enq_y_def
-  rb_enq_def by simp
-
-
-text \<open>
-  Secondly, we can show that if the head of the ring contains some buffer $b$, then 
-  just incrementing the head pointer, results in an equivalent state as when we
-  enqueue this buffer. Note, due to the definitions of reading the head element, 
-  we need to have an additional assumption, that the head is actually not none. 
-
-  We show that writing the head with the same element that currently there, yields the
-  same state. Note, this is trivial, but a proof is required due to the definition of
-  the read operation.
-\<close>
-
-lemma CleanQ_RB_write_head_x_equiv[simp]:
-assumes notnone: "\<not>CleanQ_RB_head_none_x rb"  and buf: "b = (CleanQ_RB_read_head_x rb)"
-  shows "CleanQ_RB_write_head_x b rb = rb"
-  using assms 
-  unfolding CleanQ_RB_write_head_x_def CleanQ_RB_head_none_x_def CleanQ_RB_read_head_x_def
-  by (simp add: rb_write_head_same)
-
-lemma CleanQ_RB_write_head_y_equiv[simp]:
-assumes notnone: "\<not>CleanQ_RB_head_none_y rb"  and buf: "b = (CleanQ_RB_read_head_y rb)"
-  shows "CleanQ_RB_write_head_y b rb = rb"
-  using assms 
-  unfolding CleanQ_RB_write_head_y_def CleanQ_RB_head_none_y_def CleanQ_RB_read_head_y_def
-  by (simp add: rb_write_head_same)
-
-
-text \<open>
-  Using the state equivalence, we can now show that we can simply increment the head 
-  which yields the same as if we were to do a full \verb+enqueue+ operation.
-\<close>
-
-lemma CleanQ_RB_enq_x_equiv_incr_head:
-assumes notnone: "\<not>CleanQ_RB_head_none_x rb"  and buf: "b = (CleanQ_RB_read_head_x rb)"
-  shows "CleanQ_RB_incr_head_x b rb = CleanQ_RB_enq_x b rb"
-  by (metis CleanQ_RB_enq_x_split_equal CleanQ_RB_write_head_x_equiv buf notnone)
-
-lemma CleanQ_RB_enq_y_equiv_incr_head:
-assumes notnone: "\<not>CleanQ_RB_head_none_y rb"  and buf: "b = (CleanQ_RB_read_head_y rb)"
-  shows "CleanQ_RB_incr_head_y b rb = CleanQ_RB_enq_y b rb"
-  by (metis CleanQ_RB_enq_y_split_equal CleanQ_RB_write_head_y_equiv buf notnone)
-
-
-text \<open>
-  Just writing the head element in the ring, does not change the state when its lifted
-  to the list model. 
-\<close>
-
-lemma CleanQ_RB_write_head_x_list[simp]:
-  "CleanQ_RB_list (rTXY (CleanQ_RB_write_head_x b rb)) = CleanQ_RB_list (rTXY rb)"
-  by (metis CleanQ_RB_State.ext_inject CleanQ_RB_State.surjective rb_enq_write_same
-            CleanQ_RB_State.update_convs(3) CleanQ_RB_write_head_x_def)
-    
-lemma CleanQ_RB_write_head_y_list[simp]:
- "CleanQ_RB_list (rTYX (CleanQ_RB_write_head_y b rb)) = CleanQ_RB_list (rTYX rb)"
-  by (metis CleanQ_RB_State.ext_inject CleanQ_RB_State.surjective rb_enq_write_same
-            CleanQ_RB_State.update_convs(4) CleanQ_RB_write_head_y_def)
-
-
-text \<open>
-  The entire lifted state to the list model is not changed at all.  
-\<close>
-
-lemma CleanQ_RB_write_head_x_lift_full[simp]:
-  "CleanQ_RB2List (CleanQ_RB_write_head_x b rb) = CleanQ_RB2List rb"
-  unfolding CleanQ_RB2List_def by (simp, auto simp: CleanQ_RB_write_head_x_def)
-
-lemma CleanQ_RB_write_head_y_lift_full[simp]:
-  "CleanQ_RB2List (CleanQ_RB_write_head_y b rb) = CleanQ_RB2List rb"
-  unfolding CleanQ_RB2List_def by (simp, auto simp: CleanQ_RB_write_head_y_def)
-
-
-text \<open>
-  Writing the head preserves all \verb+can_enq+ and \verb+can_deq+ predicates. 
-\<close>
-
-lemma CleanQ_RB_write_head_y_can_enq_x[simp]:
-  "CleanQ_RB_enq_x_possible (CleanQ_RB_write_head_y b rb) = CleanQ_RB_enq_x_possible rb"
-  by (simp add: CleanQ_RB_write_head_y_def CleanQ_RB_enq_x_possible_def) 
-
-lemma CleanQ_RB_write_head_y_can_deq_y[simp]:
-  "CleanQ_RB_deq_y_possible (CleanQ_RB_write_head_y b rb) = CleanQ_RB_deq_y_possible rb"
-  by (simp add: CleanQ_RB_deq_y_possible_def CleanQ_RB_write_head_y_def)
-
-lemma CleanQ_RB_write_head_y_can_deq_x[simp]:
- "CleanQ_RB_deq_x_possible (CleanQ_RB_write_head_y b rb) = CleanQ_RB_deq_x_possible rb"
-  by(simp add: CleanQ_RB_deq_x_possible_def CleanQ_RB_write_head_y_def)
- 
-lemma CleanQ_RB_write_head_y_can_enq_y[simp]:
- "CleanQ_RB_enq_y_possible (CleanQ_RB_write_head_y b rb) = CleanQ_RB_enq_y_possible rb"
-  by(simp add: CleanQ_RB_enq_y_possible_def CleanQ_RB_write_head_y_def)
-
-
-lemma CleanQ_RB_write_head_x_can_enq_x[simp]:
-  "CleanQ_RB_enq_x_possible (CleanQ_RB_write_head_x b rb) = CleanQ_RB_enq_x_possible rb"
-  by(simp add: CleanQ_RB_write_head_x_def CleanQ_RB_enq_x_possible_def)
-
-lemma CleanQ_RB_write_head_x_can_deq_x[simp]:
- "CleanQ_RB_deq_x_possible (CleanQ_RB_write_head_x b rb) = CleanQ_RB_deq_x_possible rb"
-  by(simp add: CleanQ_RB_deq_x_possible_def CleanQ_RB_write_head_x_def)
-
-lemma CleanQ_RB_write_head_x_can_deq_y[simp]:
-  "CleanQ_RB_deq_y_possible (CleanQ_RB_write_head_x b rb) = CleanQ_RB_deq_y_possible rb"
-  by(simp add: CleanQ_RB_deq_y_possible_def CleanQ_RB_write_head_x_def)
-
-lemma CleanQ_RB_write_head_x_can_enq_y[simp]:
- "CleanQ_RB_enq_y_possible (CleanQ_RB_write_head_x b rb) = CleanQ_RB_enq_y_possible rb"
-  by(simp add: CleanQ_RB_enq_y_possible_def CleanQ_RB_write_head_x_def)
-
-
-text \<open>
-  Next we show that the write operation preserves the invariant. We show this individually, 
-  plus also we show both ways, as a simple write to the ring, does not change anything
-  in the observable state and thus also preserves the invariant.
-\<close>
-
-lemma CleanQ_RB_write_head_x_I1[simp]:
- "I1_rb_img (CleanQ_RB_write_head_x b rb) K = I1_rb_img rb K"
-  by (simp add:I1_rb_img_lift)
-
-lemma CleanQ_RB_write_head_x_I2[simp]:
- "I2_rb_img (CleanQ_RB_write_head_x b rb) = I2_rb_img rb "
-  by (simp add: I2_rb_img_lift)
-
-lemma CleanQ_RB_write_head_x_I3[simp]:
-  "I3_rb_img (CleanQ_RB_write_head_x b rb) = I3_rb_img rb"
-  by (simp add: I3_rb_img_lift)
-
-lemma CleanQ_RB_write_head_x_I4[simp]:
-  "I4_rb_valid (CleanQ_RB_write_head_x b rb) = I4_rb_valid rb"
-  unfolding I4_rb_valid_def CleanQ_RB_write_head_x_def
-  by(simp, meson rb_write_head_valid)
-
-lemma CleanQ_RB_write_head_x_Invariant[simp]:
-  "CleanQ_RB_Invariants K (CleanQ_RB_write_head_x b rb) = CleanQ_RB_Invariants K rb"
-  by (simp add: CleanQ_RB_Invariants_def)
-
-
-lemma CleanQ_RB_write_head_y_I1[simp]:
- "I1_rb_img (CleanQ_RB_write_head_y b rb) K = I1_rb_img rb K"
-  by (simp add:I1_rb_img_lift)
-
-lemma CleanQ_RB_write_head_y_I2[simp]:
- "I2_rb_img (CleanQ_RB_write_head_y b rb) = I2_rb_img rb"
-  by (simp add: I2_rb_img_lift)
-
-lemma CleanQ_RB_write_head_y_I3[simp]:
-  "I3_rb_img (CleanQ_RB_write_head_y b rb) = I3_rb_img rb"
-  by (simp add: I3_rb_img_lift)
-
-lemma CleanQ_RB_write_head_y_I4[simp]:
-  "I4_rb_valid (CleanQ_RB_write_head_y b rb) = I4_rb_valid rb"
-  unfolding I4_rb_valid_def CleanQ_RB_write_head_y_def
-  by(simp, meson rb_write_head_valid)
-
-lemma CleanQ_RB_write_head_y_Invariant[simp]:
-  "CleanQ_RB_Invariants K rb \<longleftrightarrow> CleanQ_RB_Invariants K (CleanQ_RB_write_head_y b rb)"
-  by (simp add:CleanQ_RB_Invariants_def)
-
-(* ------------------------------------------------------------------------------------ *)
-subsubsection \<open>Dequeue Operation\<close>
-(* ------------------------------------------------------------------------------------ *)
-
-text \<open>
-  The first part of the \verb+dequeue+ operation is to read from the ring buffer to 
-  obtain the element to be dequeued. Note, if the ring is not empty, there is always some
-  element to be dequeued.
-\<close>
-
-definition CleanQ_RB_read_tail_x :: "'a CleanQ_RB_State \<Rightarrow> 'a " 
-  where "CleanQ_RB_read_tail_x rb = rb_read_tail (rTYX rb)"
-
-definition CleanQ_RB_read_tail_y :: "'a CleanQ_RB_State \<Rightarrow> 'a " 
-  where "CleanQ_RB_read_tail_y rb = rb_read_tail (rTXY rb)"
-
-text \<open>
-  The second part is to increment the tail pointer. This effectively removes the 
-  buffer from the ring and places it into the owned set SX or SY respectively.
-\<close>
-
-definition CleanQ_RB_incr_tail_x :: "'a \<Rightarrow> 'a CleanQ_RB_State \<Rightarrow> 'a CleanQ_RB_State" 
-  where "CleanQ_RB_incr_tail_x b rb = rb \<lparr>rTYX := rb_incr_tail (rTYX rb), 
-                                          rSX := (rSX rb) \<union> {b} \<rparr>"
-
-definition CleanQ_RB_incr_tail_y :: "'a \<Rightarrow> 'a CleanQ_RB_State \<Rightarrow> 'a CleanQ_RB_State" 
-  where "CleanQ_RB_incr_tail_y b rb = rb \<lparr>rTXY := rb_incr_tail (rTXY rb), 
-                                          rSY := (rSY rb) \<union> {b} \<rparr>"
-
-
-text \<open>
-  We define helper functions to check  whether the head position of the ring is 
-  \verb+None+ or it contains some buffer.
-\<close>
-
-definition CleanQ_RB_tail_none_x :: "'a CleanQ_RB_State \<Rightarrow> bool" 
-  where "CleanQ_RB_tail_none_x rb = rb_tail_none (rTXY rb)"
-
-definition CleanQ_RB_tail_none_y :: "'a CleanQ_RB_State \<Rightarrow> bool" 
-  where "CleanQ_RB_tail_none_y rb = rb_tail_none (rTYX rb)"
-
-
-text \<open>
-  We first show, that the combination of the two operations yields the original 
-  \verb+dequeue+ operation of the sequential ring buffer model. We add those two to 
-  the simp set.
-\<close>
-
-lemma CleanQ_split_deq_x_equal[simp]:
-  "CleanQ_RB_incr_tail_x (CleanQ_RB_read_tail_x rb) rb = CleanQ_RB_deq_x rb"
-  unfolding CleanQ_RB_deq_x_def rb_deq_def CleanQ_RB_read_tail_x_def CleanQ_RB_incr_tail_x_def
-  by simp
-
-lemma CleanQ_split_deq_y_equal[simp]:
-  "CleanQ_RB_incr_tail_y (CleanQ_RB_read_tail_y rb) rb = CleanQ_RB_deq_y rb"
-  unfolding CleanQ_RB_deq_y_def rb_deq_def CleanQ_RB_read_tail_y_def CleanQ_RB_incr_tail_y_def
-  by simp
-
-
-text \<open>
-  Secondly, we show that if the buffer at tail is $b$ then incrementing the head yields
-  the same outcome as the dequeue operation.
-\<close>
-
-lemma CleanQ_RB_deq_x_equiv_incr_tail:
-  "b = (CleanQ_RB_read_tail_x rb) \<Longrightarrow> CleanQ_RB_incr_tail_x b rb = CleanQ_RB_deq_x rb"
-  by(simp)
-
-lemma CleanQ_RB_deq_y_equiv_incr_tail:
-  "b = (CleanQ_RB_read_tail_y rb) \<Longrightarrow> CleanQ_RB_incr_tail_y b rb = CleanQ_RB_deq_y rb"
-  by(simp)
-  
 (* ------------------------------------------------------------------------------------ *)
 subsubsection \<open>Weak frame condition preserver invariants\<close>
 (* ------------------------------------------------------------------------------------ *)
@@ -714,4 +380,578 @@ lemma CleanQ_CRB_frame_y_I_all :
   using assms unfolding frame_rb_weak_y_def CleanQ_RB_Invariants_def
   by (meson CleanQ_CRB_frame_y_I1 CleanQ_CRB_frame_y_I2 CleanQ_CRB_frame_y_I3 CleanQ_CRB_frame_y_I4 
       frame invariants)
+
+
+(* ==================================================================================== *)
+subsection \<open>State Transition Operations\<close>
+(* ==================================================================================== *)
+
+text \<open>
+  We now formulate the state transition operations in terms of the CleanQ RB model
+  state. Again, the two agents can, independently from each other, perform one of 
+  two operations, \verb+enqueue+ and \verb+dequeue+,  which trigger an ownership 
+  transfer of buffer elements. In the previous model we implemented \verb+enqueue+ and
+  \verb+dequeue+ as a single atomic step. Here we define it as two steps each.   
+
+  We will first show that the enqueue and dequeue operations in two calls are
+  the same as the atomic step and also preserve the invariant. This is basically
+  showing equivalence in the non concurrent setting
+\<close>
+
+(* ------------------------------------------------------------------------------------ *)
+subsubsection \<open>Enqueue Operation\<close>
+(* ------------------------------------------------------------------------------------ *)
+
+text \<open>
+  The first part of the \verb+enqueue+ operation is to write head buffer element into
+  the ring at the head position.
+\<close>
+
+definition CleanQ_RB_write_head_x :: "'a \<Rightarrow> 'a CleanQ_RB_State \<Rightarrow> 'a CleanQ_RB_State" 
+  where "CleanQ_RB_write_head_x b rb = rb \<lparr>rTXY := rb_write_head b (rTXY rb) \<rparr>"
+
+definition CleanQ_RB_write_head_y :: "'a \<Rightarrow> 'a CleanQ_RB_State \<Rightarrow> 'a CleanQ_RB_State" 
+  where "CleanQ_RB_write_head_y b rb = rb \<lparr>rTYX := rb_write_head b (rTYX rb) \<rparr>"
+
+text \<open>
+  The second part is to increment the head pointer, this effectively transfers the 
+  ownership of the buffer from the owning sets SX or SY to the transfer set TXY or TYX. 
+\<close>
+
+definition CleanQ_RB_incr_head_x :: "'a \<Rightarrow> 'a CleanQ_RB_State \<Rightarrow> 'a CleanQ_RB_State" 
+  where "CleanQ_RB_incr_head_x b rb = rb \<lparr>rTXY := rb_incr_head (rTXY rb), 
+                                          rSX := (rSX rb) - {b} \<rparr>"
+
+definition CleanQ_RB_incr_head_y :: "'a \<Rightarrow> 'a CleanQ_RB_State \<Rightarrow> 'a CleanQ_RB_State" 
+  where "CleanQ_RB_incr_head_y b rb = rb \<lparr> rTYX := rb_incr_head (rTYX rb), 
+                                           rSY := (rSY rb) - {b} \<rparr>"
+
+
+text \<open>
+  We define helper functions to read the head pointer of the ring buffer and to check
+  whether the head position of the ring is \verb+None+ or it contains some buffer.
+\<close>
+
+definition CleanQ_RB_read_head_x :: "'a CleanQ_RB_State \<Rightarrow> 'a " 
+  where "CleanQ_RB_read_head_x rb = rb_read_head (rTXY rb)"
+
+definition CleanQ_RB_read_head_y :: "'a CleanQ_RB_State \<Rightarrow> 'a " 
+  where "CleanQ_RB_read_head_y rb = rb_read_head (rTYX rb)"
+
+definition CleanQ_RB_head_none_x :: "'a CleanQ_RB_State \<Rightarrow> bool" 
+  where "CleanQ_RB_head_none_x rb = rb_head_none (rTXY rb)"
+
+definition CleanQ_RB_head_none_y :: "'a CleanQ_RB_State \<Rightarrow> bool" 
+  where "CleanQ_RB_head_none_y rb = rb_head_none (rTYX rb)"
+
+
+text \<open> 
+  Writing the head location in the ring ensures that the head is not none. 
+\<close>
+
+lemma CleanQ_RB_head_write_x_not_none[simp]:
+  "\<not>CleanQ_RB_head_none_x (CleanQ_RB_write_head_x b rb)"
+  unfolding CleanQ_RB_head_none_x_def CleanQ_RB_write_head_x_def
+  by (simp add: rb_write_head_not_none)
+
+lemma CleanQ_RB_head_write_y_not_none[simp]:
+  "\<not>CleanQ_RB_head_none_y (CleanQ_RB_write_head_y b rb)"
+  unfolding CleanQ_RB_head_none_y_def CleanQ_RB_write_head_y_def
+  by (simp add: rb_write_head_not_none)
+
+lemma CleanQ_RB_write_head_read_head_x[simp]:
+  "b = CleanQ_RB_read_head_x (CleanQ_RB_write_head_x b rb)"
+  unfolding CleanQ_RB_read_head_x_def CleanQ_RB_write_head_x_def
+  by (simp add: rb_read_head_def rb_write_head_element_read)
+
+lemma CleanQ_RB_write_head_read_head_y[simp]:
+  "b = CleanQ_RB_read_head_y (CleanQ_RB_write_head_y b rb)"
+  unfolding CleanQ_RB_read_head_y_def CleanQ_RB_write_head_y_def
+  by (simp add: rb_read_head_def rb_write_head_element_read)
+
+
+text \<open>
+  We first show, that the combination of the two operation, yields the original 
+  \verb+enqueue+ operation of the sequential ring buffer model. We add those two to
+  the simp set.
+\<close>
+
+lemma CleanQ_RB_enq_x_split_equal[simp]:
+  "CleanQ_RB_incr_head_x b (CleanQ_RB_write_head_x b rb) = CleanQ_RB_enq_x b rb"
+  unfolding CleanQ_RB_incr_head_x_def CleanQ_RB_write_head_x_def CleanQ_RB_enq_x_def
+  rb_enq_def by simp
+
+lemma CleanQ_RB_enq_y_split_equal[simp]:
+  "CleanQ_RB_incr_head_y b (CleanQ_RB_write_head_y b rb) = CleanQ_RB_enq_y b rb"
+  unfolding CleanQ_RB_incr_head_y_def CleanQ_RB_write_head_y_def CleanQ_RB_enq_y_def
+  rb_enq_def by simp
+
+
+text \<open>
+  Secondly, we can show that if the head of the ring contains some buffer $b$, then 
+  just incrementing the head pointer, results in an equivalent state as when we
+  enqueue this buffer. Note, due to the definitions of reading the head element, 
+  we need to have an additional assumption, that the head is actually not none. 
+
+  We show that writing the head with the same element that currently there, yields the
+  same state. Note, this is trivial, but a proof is required due to the definition of
+  the read operation.
+\<close>
+
+lemma CleanQ_RB_write_head_x_equiv[simp]:
+assumes notnone: "\<not>CleanQ_RB_head_none_x rb"  and buf: "b = (CleanQ_RB_read_head_x rb)"
+  shows "CleanQ_RB_write_head_x b rb = rb"
+  using assms 
+  unfolding CleanQ_RB_write_head_x_def CleanQ_RB_head_none_x_def CleanQ_RB_read_head_x_def
+  by (simp add: rb_write_head_same)
+
+lemma CleanQ_RB_write_head_y_equiv[simp]:
+assumes notnone: "\<not>CleanQ_RB_head_none_y rb"  and buf: "b = (CleanQ_RB_read_head_y rb)"
+  shows "CleanQ_RB_write_head_y b rb = rb"
+  using assms 
+  unfolding CleanQ_RB_write_head_y_def CleanQ_RB_head_none_y_def CleanQ_RB_read_head_y_def
+  by (simp add: rb_write_head_same)
+
+
+text \<open>
+  Using the state equivalence, we can now show that we can simply increment the head 
+  which yields the same as if we were to do a full \verb+enqueue+ operation.
+\<close>
+
+lemma CleanQ_RB_enq_x_equiv_incr_head[simp]:
+assumes notnone: "\<not>CleanQ_RB_head_none_x rb"  and buf: "b = (CleanQ_RB_read_head_x rb)"
+  shows "CleanQ_RB_incr_head_x b rb = CleanQ_RB_enq_x b rb"
+  by (metis CleanQ_RB_enq_x_split_equal CleanQ_RB_write_head_x_equiv buf notnone)
+
+lemma CleanQ_RB_enq_y_equiv_incr_head[simp]:
+assumes notnone: "\<not>CleanQ_RB_head_none_y rb"  and buf: "b = (CleanQ_RB_read_head_y rb)"
+  shows "CleanQ_RB_incr_head_y b rb = CleanQ_RB_enq_y b rb"
+  by (metis CleanQ_RB_enq_y_split_equal CleanQ_RB_write_head_y_equiv buf notnone)
+
+
+text \<open>
+  Just writing the head element in the ring, does not change the state when its lifted
+  to the list model. 
+\<close>
+
+lemma CleanQ_RB_write_head_x_list[simp]:
+  "CleanQ_RB_list (rTXY (CleanQ_RB_write_head_x b rb)) = CleanQ_RB_list (rTXY rb)"
+  by (metis CleanQ_RB_State.ext_inject CleanQ_RB_State.surjective rb_enq_write_same
+            CleanQ_RB_State.update_convs(3) CleanQ_RB_write_head_x_def)
+    
+lemma CleanQ_RB_write_head_y_list[simp]:
+ "CleanQ_RB_list (rTYX (CleanQ_RB_write_head_y b rb)) = CleanQ_RB_list (rTYX rb)"
+  by (metis CleanQ_RB_State.ext_inject CleanQ_RB_State.surjective rb_enq_write_same
+            CleanQ_RB_State.update_convs(4) CleanQ_RB_write_head_y_def)
+
+
+text \<open>
+  The entire lifted state to the list model is not changed at all.  
+\<close>
+
+lemma CleanQ_RB_write_head_x_lift_full[simp]:
+  "CleanQ_RB2List (CleanQ_RB_write_head_x b rb) = CleanQ_RB2List rb"
+  unfolding CleanQ_RB2List_def by (simp, auto simp: CleanQ_RB_write_head_x_def)
+
+lemma CleanQ_RB_write_head_y_lift_full[simp]:
+  "CleanQ_RB2List (CleanQ_RB_write_head_y b rb) = CleanQ_RB2List rb"
+  unfolding CleanQ_RB2List_def by (simp, auto simp: CleanQ_RB_write_head_y_def)
+
+
+text \<open>
+  Writing the head preserves all \verb+can_enq+ and \verb+can_deq+ predicates. 
+\<close>
+
+lemma CleanQ_RB_write_head_y_can_enq_x[simp]:
+  "CleanQ_RB_enq_x_possible (CleanQ_RB_write_head_y b rb) = CleanQ_RB_enq_x_possible rb"
+  by (simp add: CleanQ_RB_write_head_y_def CleanQ_RB_enq_x_possible_def) 
+
+lemma CleanQ_RB_write_head_y_can_deq_y[simp]:
+  "CleanQ_RB_deq_y_possible (CleanQ_RB_write_head_y b rb) = CleanQ_RB_deq_y_possible rb"
+  by (simp add: CleanQ_RB_deq_y_possible_def CleanQ_RB_write_head_y_def)
+
+lemma CleanQ_RB_write_head_y_can_deq_x[simp]:
+ "CleanQ_RB_deq_x_possible (CleanQ_RB_write_head_y b rb) = CleanQ_RB_deq_x_possible rb"
+  by(simp add: CleanQ_RB_deq_x_possible_def CleanQ_RB_write_head_y_def)
+ 
+lemma CleanQ_RB_write_head_y_can_enq_y[simp]:
+ "CleanQ_RB_enq_y_possible (CleanQ_RB_write_head_y b rb) = CleanQ_RB_enq_y_possible rb"
+  by(simp add: CleanQ_RB_enq_y_possible_def CleanQ_RB_write_head_y_def)
+
+
+lemma CleanQ_RB_write_head_x_can_enq_x[simp]:
+  "CleanQ_RB_enq_x_possible (CleanQ_RB_write_head_x b rb) = CleanQ_RB_enq_x_possible rb"
+  by(simp add: CleanQ_RB_write_head_x_def CleanQ_RB_enq_x_possible_def)
+
+lemma CleanQ_RB_write_head_x_can_deq_x[simp]:
+ "CleanQ_RB_deq_x_possible (CleanQ_RB_write_head_x b rb) = CleanQ_RB_deq_x_possible rb"
+  by(simp add: CleanQ_RB_deq_x_possible_def CleanQ_RB_write_head_x_def)
+
+lemma CleanQ_RB_write_head_x_can_deq_y[simp]:
+  "CleanQ_RB_deq_y_possible (CleanQ_RB_write_head_x b rb) = CleanQ_RB_deq_y_possible rb"
+  by(simp add: CleanQ_RB_deq_y_possible_def CleanQ_RB_write_head_x_def)
+
+lemma CleanQ_RB_write_head_x_can_enq_y[simp]:
+ "CleanQ_RB_enq_y_possible (CleanQ_RB_write_head_x b rb) = CleanQ_RB_enq_y_possible rb"
+  by(simp add: CleanQ_RB_enq_y_possible_def CleanQ_RB_write_head_x_def)
+
+
+text \<open>
+  Also, other sets are not affected when writing the head buffer element 
+\<close>
+
+lemma CleanQ_RB_write_head_y_SX[simp]:
+  "rSX (CleanQ_RB_write_head_y b rb) = rSX rb"
+  unfolding CleanQ_RB_write_head_y_def by(auto)
+
+lemma CleanQ_RB_write_head_y_SY[simp]:
+  "rSY (CleanQ_RB_write_head_y b rb) = rSY rb"
+  unfolding CleanQ_RB_write_head_y_def by(auto)
+
+lemma CleanQ_RB_write_head_x_SX[simp]:
+  "rSX (CleanQ_RB_write_head_x b rb) = rSX rb"
+  unfolding CleanQ_RB_write_head_x_def by(auto)
+
+lemma CleanQ_RB_write_head_x_SY[simp]:
+  "rSY (CleanQ_RB_write_head_x b rb) = rSY rb"
+  unfolding CleanQ_RB_write_head_x_def by(auto)
+
+
+text \<open>
+  Next we show that the write operation preserves the invariant. We show this individually, 
+  plus also we show both ways, as a simple write to the ring, does not change anything
+  in the observable state and thus also preserves the invariant.
+\<close>
+
+lemma CleanQ_RB_write_head_x_I1[simp]:
+ "I1_rb_img (CleanQ_RB_write_head_x b rb) K = I1_rb_img rb K"
+  by (simp add:I1_rb_img_lift)
+
+lemma CleanQ_RB_write_head_x_I2[simp]:
+ "I2_rb_img (CleanQ_RB_write_head_x b rb) = I2_rb_img rb "
+  by (simp add: I2_rb_img_lift)
+
+lemma CleanQ_RB_write_head_x_I3[simp]:
+  "I3_rb_img (CleanQ_RB_write_head_x b rb) = I3_rb_img rb"
+  by (simp add: I3_rb_img_lift)
+
+lemma CleanQ_RB_write_head_x_I4[simp]:
+  "I4_rb_valid (CleanQ_RB_write_head_x b rb) = I4_rb_valid rb"
+  unfolding I4_rb_valid_def CleanQ_RB_write_head_x_def
+  by(simp, meson rb_write_head_valid)
+
+lemma CleanQ_RB_write_head_x_Invariant[simp]:
+  "CleanQ_RB_Invariants K (CleanQ_RB_write_head_x b rb) = CleanQ_RB_Invariants K rb"
+  by (simp add: CleanQ_RB_Invariants_def)
+
+
+lemma CleanQ_RB_write_head_y_I1[simp]:
+ "I1_rb_img (CleanQ_RB_write_head_y b rb) K = I1_rb_img rb K"
+  by (simp add:I1_rb_img_lift)
+
+lemma CleanQ_RB_write_head_y_I2[simp]:
+ "I2_rb_img (CleanQ_RB_write_head_y b rb) = I2_rb_img rb"
+  by (simp add: I2_rb_img_lift)
+
+lemma CleanQ_RB_write_head_y_I3[simp]:
+  "I3_rb_img (CleanQ_RB_write_head_y b rb) = I3_rb_img rb"
+  by (simp add: I3_rb_img_lift)
+
+lemma CleanQ_RB_write_head_y_I4[simp]:
+  "I4_rb_valid (CleanQ_RB_write_head_y b rb) = I4_rb_valid rb"
+  unfolding I4_rb_valid_def CleanQ_RB_write_head_y_def
+  by(simp, meson rb_write_head_valid)
+
+lemma CleanQ_RB_write_head_y_Invariant[simp]:
+  "CleanQ_RB_Invariants K (CleanQ_RB_write_head_y b rb) = CleanQ_RB_Invariants K rb"
+  by (simp add:CleanQ_RB_Invariants_def)
+
+
+
+(* ------------------------------------------------------------------------------------ *)
+subsubsection \<open>Pre-Post Conditions for the Enqueue Operation\<close>
+(* ------------------------------------------------------------------------------------ *)
+
+
+text \<open>
+  We now define the hoare triples for the enqueue operation. Those are needed to later
+  for the interference proof. There are a total of three predicates for the enqueue
+  operation in small step semantics, while the predicates P and R define the big 
+  step semantics.
+
+  \verb+{P} write_head {Q} incr_head {R}+ 
+
+  We now provide abbreviations for each of the predicate P, Q, and R for the \verb+enqueue+
+  operation as seen from Y and X.   
+\<close>
+
+paragraph \<open>Enqueue P\<close>
+
+text \<open>
+  The P predicate is the pre-condition for the \verb+enqueue+ operation. For the operation
+  to succeed, the state must satisfy the Invariant plus an enqueue must be possible, i.e.
+  there is space in the descriptor ring to hold the buffer. Lastly, the buffer to be 
+  enqueued must be owned by the agent i.e. a member of the set SX or SY respectively.
+  We provide two abbreviations for this, one for each side:\<close>
+
+abbreviation "CleanQ_RB_enq_x_P K rb b \<equiv> CleanQ_RB_Invariants K rb \<and> 
+                                          CleanQ_RB_enq_x_possible rb \<and> b \<in> rSX rb"
+
+abbreviation "CleanQ_RB_enq_y_P K rb b \<equiv> CleanQ_RB_Invariants K rb \<and> 
+                                          CleanQ_RB_enq_y_possible rb \<and> b \<in> rSY rb"
+
+paragraph \<open>Enqueue Q\<close>
+
+text \<open>
+  The Q predicate is the post-condition for the write part of the  \verb+enqueue+ operation, 
+  and the pre-condition of the increment part of the \verb+enqueue+ operation. The write
+  operation does not transfer ownership of the buffer yet, thus the buffer remains in
+  SX or SY respectively and the enqueue still remains possible. However, we now know, 
+  that the buffer is written to the head location of the ring, and that this location
+  is not \verb+None+.
+\<close>
+
+abbreviation "CleanQ_RB_enq_x_Q K rb b \<equiv> CleanQ_RB_Invariants K rb \<and> 
+                                          CleanQ_RB_enq_x_possible rb \<and> b \<in> rSX rb \<and> 
+                                          b = CleanQ_RB_read_head_x rb \<and> 
+                                          \<not>CleanQ_RB_head_none_x rb "
+
+abbreviation "CleanQ_RB_enq_y_Q K rb b \<equiv> CleanQ_RB_Invariants K rb \<and> 
+                                          CleanQ_RB_enq_y_possible rb \<and> b \<in> rSY rb \<and>
+                                           b = CleanQ_RB_read_head_y rb \<and> 
+                                           \<not>CleanQ_RB_head_none_y rb "
+
+paragraph \<open>Enqueue R\<close>
+
+
+text \<open>
+  The R predicate is the post condition for both, the increment head part as well as the
+  full \verb+enqueue+ operation. We now that the buffer is now no longer in the owning 
+  sets SX and SY. Note, we cannot make a state about whether it is in the ring, because
+  the other side may have already taken it out. Also, we cannot make any statements
+  about whether we can enqueue again.
+\<close>
+
+abbreviation "CleanQ_RB_enq_y_R K rb b \<equiv> CleanQ_RB_Invariants K rb \<and> b \<notin> rSX rb"
+
+abbreviation "CleanQ_RB_enq_x_R K rb b \<equiv> CleanQ_RB_Invariants K rb \<and> b \<notin> rSY rb"
+
+
+(* ------------------------------------------------------------------------------------ *)
+subsubsection \<open>Dequeue Operation\<close>
+(* ------------------------------------------------------------------------------------ *)
+
+text \<open>
+  The first part of the \verb+dequeue+ operation is to read from the ring buffer to 
+  obtain the element to be dequeued. Note, if the ring is not empty, there is always some
+  element to be dequeued.
+\<close>
+
+definition CleanQ_RB_read_tail_x :: "'a CleanQ_RB_State \<Rightarrow> 'a " 
+  where "CleanQ_RB_read_tail_x rb = rb_read_tail (rTYX rb)"
+
+definition CleanQ_RB_read_tail_y :: "'a CleanQ_RB_State \<Rightarrow> 'a " 
+  where "CleanQ_RB_read_tail_y rb = rb_read_tail (rTXY rb)"
+
+text \<open>
+  The second part is to increment the tail pointer. This effectively removes the 
+  buffer from the ring and places it into the owned set SX or SY respectively.
+\<close>
+
+definition CleanQ_RB_incr_tail_x :: "'a \<Rightarrow> 'a CleanQ_RB_State \<Rightarrow> 'a CleanQ_RB_State" 
+  where "CleanQ_RB_incr_tail_x b rb = rb \<lparr>rTYX := rb_incr_tail (rTYX rb), 
+                                          rSX := (rSX rb) \<union> {b} \<rparr>"
+
+definition CleanQ_RB_incr_tail_y :: "'a \<Rightarrow> 'a CleanQ_RB_State \<Rightarrow> 'a CleanQ_RB_State" 
+  where "CleanQ_RB_incr_tail_y b rb = rb \<lparr>rTXY := rb_incr_tail (rTXY rb), 
+                                          rSY := (rSY rb) \<union> {b} \<rparr>"
+
+
+text \<open>
+  We define helper functions to check  whether the head position of the ring is 
+  \verb+None+ or it contains some buffer.
+\<close>
+
+definition CleanQ_RB_tail_none_x :: "'a CleanQ_RB_State \<Rightarrow> bool" 
+  where "CleanQ_RB_tail_none_x rb = rb_tail_none (rTXY rb)"
+
+definition CleanQ_RB_tail_none_y :: "'a CleanQ_RB_State \<Rightarrow> bool" 
+  where "CleanQ_RB_tail_none_y rb = rb_tail_none (rTYX rb)"
+
+
+text \<open>
+  We first show, that the combination of the two operations yields the original 
+  \verb+dequeue+ operation of the sequential ring buffer model. We add those two to 
+  the simp set.
+\<close>
+
+lemma CleanQ_split_deq_x_equal[simp]:
+  "CleanQ_RB_incr_tail_x (CleanQ_RB_read_tail_x rb) rb = CleanQ_RB_deq_x rb"
+  unfolding CleanQ_RB_deq_x_def rb_deq_def CleanQ_RB_read_tail_x_def CleanQ_RB_incr_tail_x_def
+  by simp
+
+lemma CleanQ_split_deq_y_equal[simp]:
+  "CleanQ_RB_incr_tail_y (CleanQ_RB_read_tail_y rb) rb = CleanQ_RB_deq_y rb"
+  unfolding CleanQ_RB_deq_y_def rb_deq_def CleanQ_RB_read_tail_y_def CleanQ_RB_incr_tail_y_def
+  by simp
+
+
+text \<open>
+  Secondly, we show that if the buffer at tail is $b$ then incrementing the head yields
+  the same outcome as the dequeue operation.
+\<close>
+
+lemma CleanQ_RB_deq_x_equiv_incr_tail:
+  "b = (CleanQ_RB_read_tail_x rb) \<Longrightarrow> CleanQ_RB_incr_tail_x b rb = CleanQ_RB_deq_x rb"
+  by(simp)
+
+lemma CleanQ_RB_deq_y_equiv_incr_tail:
+  "b = (CleanQ_RB_read_tail_y rb) \<Longrightarrow> CleanQ_RB_incr_tail_y b rb = CleanQ_RB_deq_y rb"
+  by(simp)
+
+
+text \<open>
+  The head element is not changed by the dequeue operation, thus the head element remains
+  the same, either it is Some or it is None.
+\<close>
+
+(* TODO:  create a few lemmas in CleanQ_RB so there is no need to unfold rb_ * *)
+
+lemma CleanQ_RB_read_head_x_deq_y_equiv[simp]:
+  "CleanQ_RB_read_head_x (CleanQ_RB_deq_y rb) =  CleanQ_RB_read_head_x rb"
+  unfolding CleanQ_RB_read_head_x_def CleanQ_RB_deq_y_def rb_read_head_def rb_deq_def
+            rb_incr_tail_def
+  by(auto)
+
+lemma CleanQ_RB_read_head_y_deq_x_equiv[simp]:
+  "CleanQ_RB_read_head_y (CleanQ_RB_deq_x rb) =  CleanQ_RB_read_head_y rb"
+  unfolding CleanQ_RB_read_head_y_def CleanQ_RB_deq_x_def rb_read_head_def rb_deq_def
+            rb_incr_tail_def
+  by(auto)
+
+lemma CleanQ_RB_head_non_x_deq_y[simp]:
+ "CleanQ_RB_head_none_x (CleanQ_RB_deq_y rb) = CleanQ_RB_head_none_x rb"
+  unfolding CleanQ_RB_deq_y_def rb_read_head_def rb_deq_def rb_incr_tail_def 
+            CleanQ_RB_head_none_x_def rb_head_none_def
+  by(auto)
+
+lemma CleanQ_RB_head_non_y_deq_x[simp]:
+ "CleanQ_RB_head_none_y (CleanQ_RB_deq_x rb) = CleanQ_RB_head_none_y rb"
+  unfolding CleanQ_RB_deq_x_def rb_read_head_def rb_deq_def rb_incr_tail_def 
+            CleanQ_RB_head_none_y_def rb_head_none_def
+  by(auto)
+
+text \<open>
+  The head element is not changed by the dequeue operation, thus the head element remains
+  the same, either it is Some or it is None.
+\<close>
+
+(* TODO: add a few lemmas to avoid unfolidng rb_* *)
+
+lemma CleanQ_RB_read_tail_x_write_head_x[simp]:
+ " CleanQ_RB_deq_x_possible rb \<Longrightarrow>
+  CleanQ_RB_read_tail_x (CleanQ_RB_write_head_y b rb) = CleanQ_RB_read_tail_x rb"
+  unfolding CleanQ_RB_read_tail_x_def CleanQ_RB_write_head_y_def CleanQ_RB_deq_x_possible_def
+  by (simp add: rb_can_deq_def rb_empty_def rb_read_tail_def rb_write_head_def)
+
+lemma CleanQ_RB_read_tail_y_write_head_x[simp]:
+ " CleanQ_RB_deq_y_possible rb \<Longrightarrow>
+  CleanQ_RB_read_tail_y (CleanQ_RB_write_head_x b rb) = CleanQ_RB_read_tail_y rb"
+  unfolding CleanQ_RB_read_tail_y_def CleanQ_RB_write_head_x_def CleanQ_RB_deq_y_possible_def
+  by (simp add: rb_can_deq_def rb_empty_def rb_read_tail_def rb_write_head_def)
+
+text \<open>
+  Reading the tail after an enqueue yeilds the same result
+\<close>
+
+lemma CleanQ_RB_read_tail_x_enq_y[simp]:
+  "CleanQ_RB_deq_x_possible rb \<Longrightarrow> 
+   CleanQ_RB_read_tail_x (CleanQ_RB_enq_y b rb) = CleanQ_RB_read_tail_x rb"
+  unfolding CleanQ_RB_read_tail_x_def CleanQ_RB_write_head_y_def CleanQ_RB_enq_y_def
+  unfolding rb_read_tail_def rb_write_head_def rb_enq_def rb_incr_head_def
+  by (simp add: CleanQ_RB_deq_x_possible_def rb_can_deq_def rb_empty_def)
+
+lemma CleanQ_RB_read_tail_y_enq_x[simp]:
+  "CleanQ_RB_deq_y_possible rb \<Longrightarrow> 
+   CleanQ_RB_read_tail_y (CleanQ_RB_enq_x b rb) = CleanQ_RB_read_tail_y rb"
+  unfolding CleanQ_RB_read_tail_y_def CleanQ_RB_write_head_x_def CleanQ_RB_enq_x_def
+  unfolding rb_read_tail_def rb_write_head_def rb_enq_def rb_incr_head_def
+  by (simp add: CleanQ_RB_deq_y_possible_def rb_can_deq_def rb_empty_def)
+
+
+(* ------------------------------------------------------------------------------------ *)
+subsubsection \<open>Pre-Post Conditions for the Dequeue Operation\<close>
+(* ------------------------------------------------------------------------------------ *)
+
+text \<open>
+  We now define the hoare triples for the dequeue operation. Those are needed to later
+  for the interference proof. There are a total of three predicates for the dequeue
+  operation in small step semantics, while the predicates P and R define the big 
+  step semantics.
+
+  \verb+{P} read_tail {Q} incr_tail {R}+ 
+
+  We now provide abbreviations for each of the predicate P, Q, and R for the \verb+dequeue+
+  operation as seen from Y and X.   
+\<close>
+
+
+paragraph \<open>Dequeue P\<close>
+
+text \<open>
+  The P predicate is the pre-condition for the \verb+dequeue+ operation. For this operation
+  to succeed, the state must satisfy teh Invariant plus a dequeue must be possible, i.e.
+  the ring must not be empty. 
+\<close>
+
+abbreviation "CleanQ_RB_deq_x_P K rb \<equiv> CleanQ_RB_Invariants K rb \<and> 
+                                        CleanQ_RB_deq_x_possible rb"
+
+abbreviation "CleanQ_RB_deq_y_P K rb \<equiv> CleanQ_RB_Invariants K rb \<and> 
+                                          CleanQ_RB_deq_y_possible rb"
+
+
+paragraph \<open>Dequeue Q\<close>
+
+text \<open>
+  The Q predicate is the post-condition of the read part of the \verb+dequeue+ operation, 
+  and the pre-condition of the increment tail part. Just reading the buffer does not
+  change the ownership of the buffer and it remains in the ownership of the ring. As
+  such, a dequeue is still possible.
+\<close>
+
+abbreviation "CleanQ_RB_deq_x_Q K rb b \<equiv> CleanQ_RB_Invariants K rb \<and> 
+                                          CleanQ_RB_deq_x_possible rb \<and> 
+                                          b = CleanQ_RB_read_tail_x rb"
+
+abbreviation "CleanQ_RB_deq_y_Q K rb b \<equiv> CleanQ_RB_Invariants K rb \<and> 
+                                          CleanQ_RB_deq_y_possible rb \<and> 
+                                          b = CleanQ_RB_read_tail_y rb"
+
+paragraph \<open>Dequeue R\<close>
+
+text \<open>
+  The R predicate is the post-condition of the \verb+dequeue+ operation in big step
+  semantics, as well as the post condition of the increment tail part. We now know
+  that the buffer is in the ownership of the subjects i.e. an eleemnt of SX or SY 
+  respectively. We now do not know whether we can dequeue again. 
+\<close>
+
+abbreviation "CleanQ_RB_deq_x_R K rb b \<equiv> CleanQ_RB_Invariants K rb \<and> b \<in> rSX rb"
+abbreviation "CleanQ_RB_deq_y_R K rb b \<equiv> CleanQ_RB_Invariants K rb \<and> b \<in> rSY rb"
+
+
+
+
+
+
+
+(* ==================================================================================== *)
+subsection \<open>Integration in COMPLEX\<close>
+(* ==================================================================================== *)
+
+text \<open>
+  Next, we can formulate the \verb+enqueue+ and \verb+dequeue+ operations in COMPLEX.
+\<close>
+
 end 
