CleanQ/CleanQ_CRBModel_Simpl.thy
@@ -42,134 +42,6 @@ record 'g CleanQ_CRB_State_vars =
   b_' :: "nat"
 (*>*)
 
-(* ------------------------------------------------------------------------------------ *)
-subsubsection \<open>Pre-Post Conditions for the Enqueue Operation\<close>
-(* ------------------------------------------------------------------------------------ *)
-
-
-text \<open>
-  We now define the hoare triples for the enqueue operation. Those are needed to later
-  for the interference proof. There are a total of three predicates for the enqueue
-  operation in small step semantics, while the predicates P and R define the big 
-  step semantics.
-
-  \verb+{P} write_head {Q} incr_head {R}+ 
-
-  We now provide abbreviations for each of the predicate P, Q, and R for the \verb+enqueue+
-  operation as seen from Y and X.   
-\<close>
-
-paragraph \<open>Enqueue P\<close>
-
-text \<open>
-  The P predicate is the pre-condition for the \verb+enqueue+ operation. For the operation
-  to succeed, the state must satisfy the Invariant plus an enqueue must be possible, i.e.
-  there is space in the descriptor ring to hold the buffer. Lastly, the buffer to be 
-  enqueued must be owned by the agent i.e. a member of the set SX or SY respectively.
-  We provide two abbreviations for this, one for each side:\<close>
-
-abbreviation "CleanQ_RB_enq_x_P K rb b \<equiv> CleanQ_RB_Invariants K rb \<and> 
-                                          CleanQ_RB_enq_x_possible rb \<and> b \<in> rSX rb"
-
-abbreviation "CleanQ_RB_enq_y_P K rb b \<equiv> CleanQ_RB_Invariants K rb \<and> 
-                                          CleanQ_RB_enq_y_possible rb \<and> b \<in> rSY rb"
-
-paragraph \<open>Enqueue Q\<close>
-
-text \<open>
-  The Q predicate is the post-condition for the write part of the  \verb+enqueue+ operation, 
-  and the pre-condition of the increment part of the \verb+enqueue+ operation. The write
-  operation does not transfer ownership of the buffer yet, thus the buffer remains in
-  SX or SY respectively and the enqueue still remains possible. However, we now know, 
-  that the buffer is written to the head location of the ring, and that this location
-  is not \verb+None+.
-\<close>
-
-abbreviation "CleanQ_RB_enq_x_Q K rb b \<equiv> CleanQ_RB_Invariants K rb \<and> 
-                                          CleanQ_RB_enq_x_possible rb \<and> b \<in> rSX rb \<and> 
-                                          b = CleanQ_RB_read_head_x rb \<and> 
-                                          \<not>CleanQ_RB_head_none_x rb "
-
-abbreviation "CleanQ_RB_enq_y_Q K rb b \<equiv> CleanQ_RB_Invariants K rb \<and> 
-                                          CleanQ_RB_enq_y_possible rb \<and> b \<in> rSY rb \<and>
-                                           b = CleanQ_RB_read_head_y rb \<and> 
-                                           \<not>CleanQ_RB_head_none_y rb "
-
-paragraph \<open>Enqueue R\<close>
-
-
-text \<open>
-  The R predicate is the post condition for both, the increment head part as well as the
-  full \verb+enqueue+ operation. We now that the buffer is now no longer in the owning 
-  sets SX and SY. Note, we cannot make a state about whether it is in the ring, because
-  the other side may have already taken it out. Also, we cannot make any statements
-  about whether we can enqueue again.
-\<close>
-
-abbreviation "CleanQ_RB_enq_y_R K rb b \<equiv> CleanQ_RB_Invariants K rb \<and> b \<notin> rSX rb"
-
-abbreviation "CleanQ_RB_enq_x_R K rb b \<equiv> CleanQ_RB_Invariants K rb \<and> b \<notin> rSY rb"
-
-(* ------------------------------------------------------------------------------------ *)
-subsubsection \<open>Pre-Post Conditions for the Dequeue Operation\<close>
-(* ------------------------------------------------------------------------------------ *)
-
-text \<open>
-  We now define the hoare triples for the dequeue operation. Those are needed to later
-  for the interference proof. There are a total of three predicates for the dequeue
-  operation in small step semantics, while the predicates P and R define the big 
-  step semantics.
-
-  \verb+{P} read_tail {Q} incr_tail {R}+ 
-
-  We now provide abbreviations for each of the predicate P, Q, and R for the \verb+dequeue+
-  operation as seen from Y and X.   
-\<close>
-
-
-paragraph \<open>Dequeue P\<close>
-
-text \<open>
-  The P predicate is the pre-condition for the \verb+dequeue+ operation. For this operation
-  to succeed, the state must satisfy teh Invariant plus a dequeue must be possible, i.e.
-  the ring must not be empty. 
-\<close>
-
-abbreviation "CleanQ_RB_deq_x_P K rb \<equiv> CleanQ_RB_Invariants K rb \<and> 
-                                        CleanQ_RB_deq_x_possible rb"
-
-abbreviation "CleanQ_RB_deq_y_P K rb \<equiv> CleanQ_RB_Invariants K rb \<and> 
-                                          CleanQ_RB_deq_y_possible rb"
-
-
-paragraph \<open>Dequeue Q\<close>
-
-text \<open>
-  The Q predicate is the post-condition of the read part of the \verb+dequeue+ operation, 
-  and the pre-condition of the increment tail part. Just reading the buffer does not
-  change the ownership of the buffer and it remains in the ownership of the ring. As
-  such, a dequeue is still possible.
-\<close>
-
-abbreviation "CleanQ_RB_deq_x_Q K rb b \<equiv> CleanQ_RB_Invariants K rb \<and> 
-                                          CleanQ_RB_deq_x_possible rb \<and> 
-                                          b = CleanQ_RB_read_tail_x rb"
-
-abbreviation "CleanQ_RB_deq_y_Q K rb b \<equiv> CleanQ_RB_Invariants K rb \<and> 
-                                          CleanQ_RB_deq_y_possible rb \<and> 
-                                          b = CleanQ_RB_read_tail_y rb"
-
-paragraph \<open>Dequeue R\<close>
-
-text \<open>
-  The R predicate is the post-condition of the \verb+dequeue+ operation in big step
-  semantics, as well as the post condition of the increment tail part. We now know
-  that the buffer is in the ownership of the subjects i.e. an eleemnt of SX or SY 
-  respectively. We now do not know whether we can dequeue again. 
-\<close>
-
-abbreviation "CleanQ_RB_deq_x_R K rb b \<equiv> CleanQ_RB_Invariants K rb \<and> b \<in> rSX rb"
-abbreviation "CleanQ_RB_deq_y_R K rb b \<equiv> CleanQ_RB_Invariants K rb \<and> b \<in> rSY rb"
 
 
 (* ------------------------------------------------------------------------------------ *)
@@ -192,21 +64,14 @@ text \<open>
 lemma  CleanQ_RB_write_head_x_hoare:
   "\<Gamma>\<turnstile> \<lbrace> CleanQ_RB_enq_x_P K \<acute>RingCRB b \<rbrace> 
         \<acute>RingCRB :== (CleanQ_RB_write_head_x b \<acute>RingCRB)
-      \<lbrace> CleanQ_RB_enq_x_Q K \<acute> RingCRB b  \<rbrace>"                                                 
-  apply(vcg, auto simp: CleanQ_RB_write_head_x_Invariant[symmetric] 
-                        CleanQ_RB_write_head_x_can_enq_x[symmetric]
-                        CleanQ_RB_write_head_read_head_x CleanQ_RB_head_write_x_not_none)
-  by(simp add: CleanQ_RB_write_head_x_def)
-
+      \<lbrace> CleanQ_RB_enq_x_Q K \<acute> RingCRB b  \<rbrace>"     
+  by(vcg, auto)
 
 lemma  CleanQ_RB_write_head_y_hoare:
   "\<Gamma>\<turnstile> \<lbrace> CleanQ_RB_enq_y_P K \<acute>RingCRB b \<rbrace> 
         \<acute>RingCRB :== (CleanQ_RB_write_head_y b \<acute>RingCRB)
       \<lbrace> CleanQ_RB_enq_y_Q K \<acute> RingCRB b  \<rbrace>"                                                 
-  apply(vcg, auto simp: CleanQ_RB_write_head_y_Invariant[symmetric] 
-                        CleanQ_RB_write_head_y_can_enq_y[symmetric]
-                        CleanQ_RB_write_head_read_head_y CleanQ_RB_head_write_y_not_none)
-  by(simp add: CleanQ_RB_write_head_y_def)
+  by(vcg, auto)
 
 
 paragraph \<open>Incrementing the Head Pointer\<close>
@@ -219,14 +84,14 @@ lemma  CleanQ_RB_incr_head_x_hoare:
   "\<Gamma>\<turnstile> \<lbrace>  CleanQ_RB_enq_x_Q K \<acute>RingCRB b \<rbrace> 
         \<acute>RingCRB :== (CleanQ_RB_incr_head_x b \<acute>RingCRB)
       \<lbrace> CleanQ_RB_enq_x_R K \<acute> RingCRB b  \<rbrace>"
-  apply(vcg, simp add: CleanQ_RB_enq_x_equiv_incr_head CleanQ_RB_enq_x_inv_all)
+  apply(vcg, auto simp:CleanQ_RB_enq_x_inv_all)
   by (simp add: CleanQ_RB_enq_x_result)
 
 lemma  CleanQ_RB_incr_head_y_hoare:
   "\<Gamma>\<turnstile> \<lbrace>  CleanQ_RB_enq_y_Q K \<acute>RingCRB b \<rbrace> 
         \<acute>RingCRB :== (CleanQ_RB_incr_head_y b \<acute>RingCRB)
       \<lbrace> CleanQ_RB_enq_y_R K \<acute> RingCRB b  \<rbrace>"
-  apply(vcg, simp add: CleanQ_RB_enq_y_equiv_incr_head CleanQ_RB_enq_y_inv_all)
+  apply(vcg, auto simp:CleanQ_RB_enq_y_inv_all)
   by (simp add: CleanQ_RB_enq_y_result)
 
 
@@ -250,6 +115,8 @@ lemma CleanQ_RB_enq_y_hoare :
         \<acute>RingCRB :== (CleanQ_RB_incr_head_y b \<acute>RingCRB)
       \<lbrace> CleanQ_RB_enq_y_R K \<acute>RingCRB b \<rbrace>"
   apply(vcg) using CleanQ_RB_enq_y_inv_all CleanQ_RB_enq_y_result by fastforce
+
+
 
 
 
@@ -330,10 +197,12 @@ lemma CleanQ_RB_deq_y_hoare :
   using CleanQ_RB_deq_y_all_inv apply blast
   by (simp add: CleanQ_RB_deq_y_result CleanQ_RB_read_tail_y_def)
 
+
+
 (* ==================================================================================== *)
 subsection \<open>Interference pairs\<close>
 (* ==================================================================================== *)
-(* ------------------------------------------------------------------------------------ *)
+
 
 text \<open>
   We are now showing the interference proofs for the different step. There are two threads
@@ -368,16 +237,13 @@ lemma CleanQ_CRB_Enqueue_X_P_write_head:
 "\<Gamma>\<turnstile> \<lbrace> CleanQ_RB_enq_x_P K \<acute>RingCRB bx  \<rbrace> 
    \<acute>RingCRB :== CleanQ_RB_write_head_y b \<acute>RingCRB 
   \<lbrace>  CleanQ_RB_enq_x_P K \<acute>RingCRB bx  \<rbrace>"
-  apply(vcg, simp add: CleanQ_RB_write_head_y_can_enq_x[symmetric] CleanQ_RB_write_head_y_Invariant[symmetric])  
-  by (simp add: CleanQ_RB_write_head_y_def)
+  by(vcg, auto)  
 
 lemma CleanQ_CRB_Enqueue_X_Q_write_head:
 "\<Gamma>\<turnstile> \<lbrace> CleanQ_RB_enq_x_Q K \<acute>RingCRB bx  \<rbrace> 
    \<acute>RingCRB :== CleanQ_RB_write_head_y b \<acute>RingCRB 
   \<lbrace>  CleanQ_RB_enq_x_Q K \<acute>RingCRB bx \<rbrace>"
-  apply(vcg, auto simp add: CleanQ_RB_write_head_y_can_enq_x[symmetric]
-                            CleanQ_RB_write_head_y_Invariant[symmetric])
- 
+  apply(vcg, auto) 
   apply (simp add: CleanQ_RB_write_head_y_def)
   apply (simp add: CleanQ_RB_read_head_x_def CleanQ_RB_write_head_y_def)
   by (simp add: CleanQ_RB_head_none_x_def CleanQ_RB_write_head_y_def)
@@ -387,8 +253,7 @@ lemma CleanQ_CRB_Enqueue_X_R_write_head:
 "\<Gamma>\<turnstile> \<lbrace> CleanQ_RB_enq_x_R K \<acute>RingCRB bx  \<rbrace> 
    \<acute>RingCRB :== CleanQ_RB_write_head_y b \<acute>RingCRB 
   \<lbrace>  CleanQ_RB_enq_x_R K \<acute>RingCRB bx \<rbrace>"
-  apply(vcg, auto simp:CleanQ_RB_write_head_y_Invariant[symmetric])  
-  by (simp add: CleanQ_RB_write_head_y_def)
+  by(vcg, auto)  
 
 
   
@@ -399,30 +264,24 @@ lemma CleanQ_CRB_Enqueue_X_P_incr_head:
 "\<Gamma>\<turnstile> \<lbrace>  rb = CleanQ_RB_write_head_y b \<acute>RingCRB \<and> b \<in> rSY \<acute>RingCRB \<and> CleanQ_RB_enq_y_possible \<acute>RingCRB \<and> CleanQ_RB_enq_x_P K rb bx  \<rbrace> 
    \<acute>RingCRB :== CleanQ_RB_incr_head_y b rb 
   \<lbrace>  CleanQ_RB_enq_x_P K \<acute>RingCRB bx  \<rbrace>"
-  apply(vcg, auto)
-    apply (meson CleanQ_RB_enq_y_inv_all CleanQ_RB_write_head_y_Invariant)
-  apply (meson CleanQ_RB_enq_y_enq_x_possible CleanQ_RB_write_head_y_Invariant CleanQ_RB_write_head_y_can_enq_x)
+  apply(vcg, auto simp:CleanQ_RB_enq_y_inv_all CleanQ_RB_enq_y_enq_x_possible)
   by (simp add: CleanQ_RB_enq_y_def CleanQ_RB_write_head_y_def)
-
+                                       
 
 lemma CleanQ_CRB_Enqueue_X_Q_incr_head:
 "\<Gamma>\<turnstile> \<lbrace>  rb = CleanQ_RB_write_head_y b \<acute>RingCRB \<and> b \<in> rSY \<acute>RingCRB \<and> CleanQ_RB_enq_y_possible \<acute>RingCRB \<and> CleanQ_RB_enq_x_Q K rb bx   \<rbrace> 
    \<acute>RingCRB :== CleanQ_RB_incr_head_y b rb 
   \<lbrace>  CleanQ_RB_enq_x_Q K \<acute>RingCRB bx \<rbrace>"
-  apply(vcg, auto)
-  apply (meson CleanQ_RB_enq_y_inv_all CleanQ_RB_write_head_y_Invariant)
-  apply (meson CleanQ_RB_enq_y_enq_x_possible CleanQ_RB_write_head_y_Invariant CleanQ_RB_write_head_y_can_enq_x)
-    apply (simp add: CleanQ_RB_enq_y_def CleanQ_RB_write_head_y_def)
-   apply (simp add: CleanQ_RB_enq_y_def CleanQ_RB_read_head_x_def CleanQ_RB_write_head_y_def)
-  by (simp add: CleanQ_RB_enq_y_def CleanQ_RB_head_none_x_def CleanQ_RB_write_head_y_def)
-  
+  apply(vcg, auto simp: CleanQ_RB_enq_y_inv_all CleanQ_RB_enq_y_enq_x_possible)
+  by(simp_all add: CleanQ_RB_enq_y_def CleanQ_RB_read_head_x_def CleanQ_RB_write_head_y_def
+                   CleanQ_RB_head_none_x_def )
+
   
 lemma CleanQ_CRB_Enqueue_X_R_incr_head:
 "\<Gamma>\<turnstile> \<lbrace> rb = CleanQ_RB_write_head_y b \<acute>RingCRB \<and> b \<in> rSY \<acute>RingCRB \<and> CleanQ_RB_enq_y_possible \<acute>RingCRB \<and> CleanQ_RB_enq_x_R K rb bx  \<rbrace> 
    \<acute>RingCRB :== CleanQ_RB_incr_head_y b rb 
   \<lbrace>  CleanQ_RB_enq_x_R K \<acute>RingCRB bx \<rbrace>"
-  apply(vcg, auto)
-  apply (meson CleanQ_RB_enq_y_inv_all CleanQ_RB_write_head_y_Invariant)
+  apply(vcg, auto simp: CleanQ_RB_enq_y_inv_all)
   by (simp add: CleanQ_RB_enq_y_def CleanQ_RB_write_head_y_def)
 
 (* ------------------------------------------------------------------------------------ *)
@@ -458,14 +317,14 @@ lemma CleanQ_CRB_Enqueue_X_P_incr_tail:
   apply(vcg, auto simp:CleanQ_RB_deq_y_all_inv CleanQ_RB_deq_y_enq_x_possible )  
   using CleanQ_RB_deq_y_no_change by blast
 
+
 lemma CleanQ_CRB_Enqueue_X_Q_incr_tail:
 "\<Gamma>\<turnstile> \<lbrace>  b = CleanQ_RB_read_tail_y  \<acute>RingCRB \<and> b \<in> rSY \<acute>RingCRB \<and> CleanQ_RB_deq_y_possible \<acute>RingCRB \<and> CleanQ_RB_enq_x_Q K \<acute>RingCRB bx  \<rbrace> 
      \<acute>RingCRB  :== CleanQ_RB_incr_tail_y b  \<acute>RingCRB 
   \<lbrace>  CleanQ_RB_enq_x_Q K \<acute>RingCRB bx \<rbrace>"
-  apply(vcg, auto simp:CleanQ_RB_deq_y_all_inv CleanQ_RB_deq_y_enq_x_possible ) 
-  using CleanQ_RB_deq_y_no_change apply blast
-  apply (metis CleanQ_RB_Invariants_def CleanQ_RB_deq_y_possible_def CleanQ_RB_read_tail_y_def I2_rb_img_def I4_rb_valid_def IntI empty_iff prod.sel(1) rb_deq_def rb_deq_list_was_in)
-  by (metis CleanQ_RB_Invariants_def CleanQ_RB_deq_y_possible_def CleanQ_RB_read_tail_y_def I2_rb_img_def I4_rb_valid_def IntI empty_iff prod.sel(1) rb_deq_def rb_deq_list_was_in)
+  apply(vcg, auto simp:CleanQ_RB_deq_y_all_inv CleanQ_RB_deq_y_enq_x_possible)
+  using CleanQ_RB_deq_y_no_change by blast
+  
 
 lemma CleanQ_CRB_Enqueue_X_R_incr_tail:
 "\<Gamma>\<turnstile> \<lbrace>  b = CleanQ_RB_read_tail_y  \<acute>RingCRB \<and> b \<in> rSY \<acute>RingCRB \<and> CleanQ_RB_deq_y_possible \<acute>RingCRB \<and> CleanQ_RB_enq_x_R K \<acute>RingCRB bx  \<rbrace> 
@@ -488,118 +347,98 @@ paragraph \<open>Y writes the descriptor ring\<close>
 lemma CleanQ_CRB_Dequeue_X_P_write_head:
 "\<Gamma>\<turnstile> \<lbrace> CleanQ_RB_deq_x_P K \<acute>RingCRB  \<rbrace> 
    \<acute>RingCRB :== CleanQ_RB_write_head_y b \<acute>RingCRB 
-  \<lbrace>  CleanQ_RB_deq_x_P K \<acute>RingCRB \<rbrace>"
-  apply(vcg)
-  by (meson CleanQ_RB_write_head_y_Invariant CleanQ_RB_write_head_y_can_deq_x)
+  \<lbrace> CleanQ_RB_deq_x_P K \<acute>RingCRB   \<rbrace>"
+  by(vcg, auto)
 
 lemma CleanQ_CRB_Dequeue_X_Q_write_head:
 "\<Gamma>\<turnstile> \<lbrace> CleanQ_RB_deq_x_Q K \<acute>RingCRB bx  \<rbrace> 
    \<acute>RingCRB :== CleanQ_RB_write_head_y b \<acute>RingCRB 
   \<lbrace>  CleanQ_RB_deq_x_Q K \<acute>RingCRB bx \<rbrace>"
-  apply(vcg, simp add: CleanQ_RB_write_head_y_can_enq_x[symmetric]
-                      CleanQ_RB_write_head_y_can_deq_x[symmetric] )
-  by (metis CleanQ_RB_Invariants_def CleanQ_RB_deq_x_possible_def
-      CleanQ_RB_read_tail_x_def CleanQ_RB_write_head_y_I4 CleanQ_RB_write_head_y_Invariant 
-      CleanQ_RB_write_head_y_can_deq_x CleanQ_RB_write_head_y_list I4_rb_valid_def prod.sel(1) 
-      rb_deq_def rb_deq_list_was_head rb_valid_implies_ptr_valid)
- 
+  by(vcg, auto)
+  
 lemma CleanQ_CRB_Dequeue_X_R_write_head:
 "\<Gamma>\<turnstile> \<lbrace> CleanQ_RB_deq_x_R K \<acute>RingCRB bx  \<rbrace> 
    \<acute>RingCRB :== CleanQ_RB_write_head_y b \<acute>RingCRB 
   \<lbrace>  CleanQ_RB_deq_x_R K \<acute>RingCRB bx \<rbrace>"
-  apply(vcg)
-  by (metis CleanQ_RB_State.ext_inject CleanQ_RB_State.surjective CleanQ_RB_State.update_convs(4) 
-      CleanQ_RB_write_head_y_Invariant CleanQ_RB_write_head_y_def)  
+  by(vcg, auto)
+
 
 paragraph \<open>Y increments the head pointer\<close>
 
 lemma CleanQ_CRB_Dequeue_X_P_incr_head:
-"\<Gamma>\<turnstile> \<lbrace>  rb = CleanQ_RB_write_head_y b \<acute>RingCRB \<and> b \<in> rSY \<acute>RingCRB \<and> CleanQ_RB_enq_y_possible \<acute>RingCRB \<and> CleanQ_RB_deq_x_P K \<acute>RingCRB \<rbrace> 
+"\<Gamma>\<turnstile> \<lbrace>  rb = CleanQ_RB_write_head_y b \<acute>RingCRB \<and> b \<in> rSY \<acute>RingCRB \<and> CleanQ_RB_enq_y_possible \<acute>RingCRB \<and> CleanQ_RB_deq_x_P K rb  \<rbrace> 
    \<acute>RingCRB :== CleanQ_RB_incr_head_y b rb 
-  \<lbrace>  CleanQ_RB_deq_x_P K \<acute>RingCRB  \<rbrace>"
-  apply(vcg)
-  by (simp add: CleanQ_RB_enq_y_deq_x_possible CleanQ_RB_enq_y_inv_all)
-  
-
+  \<lbrace>  CleanQ_RB_deq_x_P K \<acute>RingCRB   \<rbrace>"
+  by(vcg, auto simp:CleanQ_RB_enq_y_inv_all CleanQ_RB_enq_y_deq_x_possible)
   
 lemma CleanQ_CRB_Dequeue_X_Q_incr_head:
 "\<Gamma>\<turnstile> \<lbrace>  rb = CleanQ_RB_write_head_y b \<acute>RingCRB \<and> b \<in> rSY \<acute>RingCRB \<and> CleanQ_RB_enq_y_possible \<acute>RingCRB \<and> CleanQ_RB_deq_x_Q K rb bx  \<rbrace> 
    \<acute>RingCRB :== CleanQ_RB_incr_head_y b rb 
   \<lbrace>  CleanQ_RB_deq_x_Q K \<acute>RingCRB bx \<rbrace>"
-  apply(vcg, auto) 
-  apply (meson CleanQ_RB_enq_y_inv_all CleanQ_RB_write_head_y_Invariant)
-  apply (meson CleanQ_RB_enq_y_deq_x_possible CleanQ_RB_write_head_y_Invariant)
-  unfolding CleanQ_RB_read_tail_x_def CleanQ_RB_write_head_y_def CleanQ_RB_enq_y_def
-  unfolding rb_read_tail_def rb_write_head_def rb_enq_def
-  by (simp add: rb_incr_head_def)
+  by(vcg, auto simp:CleanQ_RB_enq_y_inv_all CleanQ_RB_enq_y_deq_x_possible) 
   
-
+ 
 lemma CleanQ_CRB_Dequeue_X_R_incr_head:
 "\<Gamma>\<turnstile> \<lbrace>  rb = CleanQ_RB_write_head_y b \<acute>RingCRB \<and> b \<in> rSY \<acute>RingCRB \<and> CleanQ_RB_enq_y_possible \<acute>RingCRB \<and> CleanQ_RB_deq_x_R K rb bx  \<rbrace> 
    \<acute>RingCRB :== CleanQ_RB_incr_head_y b rb 
   \<lbrace>  CleanQ_RB_deq_x_R K \<acute>RingCRB bx \<rbrace>"
-  apply(vcg)
-  by (metis CleanQ_RB_State.ext_inject CleanQ_RB_State.surjective CleanQ_RB_State.update_convs(2) 
-      CleanQ_RB_State.update_convs(4) CleanQ_RB_enq_y_inv_all CleanQ_RB_enq_y_split_equal 
-      CleanQ_RB_incr_head_y_def CleanQ_RB_write_head_y_Invariant)
-
+  apply(vcg, auto simp:CleanQ_RB_enq_y_inv_all)
+  by (simp add: CleanQ_RB_enq_y_def)
+  
+  
 (* ------------------------------------------------------------------------------------ *)
 subsubsection \<open>Dequeue X, Dequeue X\<close>
 (* ------------------------------------------------------------------------------------ *)
 
-lemma CleanQ_RB_enq_interfernce_1 :
-"\<Gamma>\<turnstile> \<lbrace> rb' = \<acute>RingCRB \<and> CleanQ_RB_Invariants K \<acute>RingCRB \<and> 
-     enq =  CleanQ_RB_enq_x_possible \<acute>RingCRB \<and> deq =  CleanQ_RB_deq_x_possible \<acute>RingCRB \<and>
-     CleanQ_RB_deq_y_possible \<acute>RingCRB \<and> enq2 = CleanQ_RB_enq_y_possible \<acute>RingCRB   \<rbrace> 
-    \<acute>b :== (CleanQ_RB_read_tail_y \<acute>RingCRB) 
-    \<lbrace> rb' = \<acute>RingCRB \<and> CleanQ_RB_Invariants K \<acute> RingCRB \<and>
-      enq =  CleanQ_RB_enq_x_possible \<acute>RingCRB \<and> deq =  CleanQ_RB_deq_x_possible \<acute>RingCRB \<and>
-     CleanQ_RB_deq_y_possible \<acute>RingCRB \<and> enq2 = CleanQ_RB_enq_y_possible \<acute>RingCRB   \<rbrace>"
+
+paragraph \<open>Y reads the descriptor ring\<close>
+
+
+lemma CleanQ_CRB_Dequeue_X_P_read_tail:
+"\<Gamma>\<turnstile> \<lbrace> CleanQ_RB_deq_x_P K \<acute>RingCRB  \<rbrace> 
+   \<acute>b :== CleanQ_RB_read_tail_y \<acute>RingCRB 
+  \<lbrace> CleanQ_RB_deq_x_P K \<acute>RingCRB   \<rbrace>"
+  by(vcg)
+
+lemma CleanQ_CRB_Dequeue_X_Q_read_tail:
+"\<Gamma>\<turnstile> \<lbrace> CleanQ_RB_deq_x_Q K \<acute>RingCRB bx  \<rbrace> 
+   \<acute>b :== CleanQ_RB_read_tail_y \<acute>RingCRB  
+  \<lbrace>  CleanQ_RB_deq_x_Q K \<acute>RingCRB bx \<rbrace>"
   by(vcg)
   
-
-lemma CleanQ_RB_enq_interfernce_2 :
-  "\<Gamma>\<turnstile> \<lbrace> rb' = \<acute>RingCRB \<and> CleanQ_RB_Invariants K \<acute> RingCRB  \<and>
-        deq =  CleanQ_RB_deq_x_possible \<acute>RingCRB \<and>
-       CleanQ_RB_deq_y_possible \<acute>RingCRB \<and> enq2 = CleanQ_RB_enq_y_possible \<acute>RingCRB  \<and>
-         b = CleanQ_RB_read_tail_y \<acute>RingCRB  \<rbrace> 
-      \<acute>RingCRB :== (CleanQ_RB_incr_tail_y b \<acute>RingCRB) 
-      \<lbrace> CleanQ_RB_Invariants K \<acute> RingCRB \<and> 
-        CleanQ_RB_enq_x_possible \<acute>RingCRB \<and> deq =  CleanQ_RB_deq_x_possible \<acute>RingCRB \<and>
-       enq2 = CleanQ_RB_enq_y_possible \<acute>RingCRB  \<and>  b \<in> rSY \<acute>RingCRB 
-       \<rbrace>"
-
-  apply (vcg, simp add: CleanQ_RB_deq_y_all_inv)
-  by(simp add: CleanQ_RB_deq_y_enq_x_possible CleanQ_RB_deq_y_deq_x_possible 
-               CleanQ_RB_deq_y_enq_y_possible CleanQ_RB_deq_y_result CleanQ_RB_read_tail_y_def)
+lemma CleanQ_CRB_Dequeue_X_R_read_tail:
+"\<Gamma>\<turnstile> \<lbrace> CleanQ_RB_deq_x_R K \<acute>RingCRB bx  \<rbrace> 
+   \<acute>b :== CleanQ_RB_read_tail_y \<acute>RingCRB 
+  \<lbrace>  CleanQ_RB_deq_x_R K \<acute>RingCRB bx \<rbrace>"
+  by(vcg)
 
 
-lemma CleanQ_RB_enq_interfernce_3 :
-    "\<Gamma>\<turnstile> \<lbrace>  rb' = \<acute>RingCRB \<and> CleanQ_RB_Invariants K \<acute> RingCRB \<and>
-           enq = CleanQ_RB_enq_x_possible \<acute>RingCRB \<and> deq =  CleanQ_RB_deq_x_possible \<acute>RingCRB \<and>
-           CleanQ_RB_enq_y_possible \<acute>RingCRB \<and> deq2 =  CleanQ_RB_deq_y_possible \<acute>RingCRB \<and>
-           b \<in> rSY \<acute>RingCRB  \<rbrace> 
-        \<acute>RingCRB :== (CleanQ_RB_write_head_y b \<acute>RingCRB)
-        \<lbrace> CleanQ_RB_Invariants K \<acute> RingCRB \<and> b \<in> rSY \<acute>RingCRB  \<and>
-         enq = CleanQ_RB_enq_x_possible \<acute>RingCRB \<and> deq =  CleanQ_RB_deq_x_possible \<acute>RingCRB \<and>
-         CleanQ_RB_enq_y_possible \<acute>RingCRB \<and> deq2 = CleanQ_RB_deq_y_possible \<acute>RingCRB \<rbrace>"
-  apply(vcg)
-  by (metis CleanQ_RB_State.ext_inject CleanQ_RB_State.surjective CleanQ_RB_State.update_convs(4) 
-      CleanQ_RB_write_head_y_Invariant CleanQ_RB_write_head_y_can_deq_x CleanQ_RB_write_head_y_can_deq_y 
-      CleanQ_RB_write_head_y_can_enq_x CleanQ_RB_write_head_y_can_enq_y CleanQ_RB_write_head_y_def)
 
-lemma CleanQ_RB_enq_interfernce_4 :
- "\<Gamma>\<turnstile> \<lbrace> rb' = \<acute>RingCRB \<and> CleanQ_RB_Invariants K \<acute> RingCRB \<and>
-        enq = CleanQ_RB_enq_x_possible \<acute>RingCRB \<and>
-        CleanQ_RB_enq_y_possible \<acute>RingCRB \<and> deq2 =  CleanQ_RB_deq_y_possible \<acute>RingCRB \<and>
-        b \<in> rSY \<acute>RingCRB \<and> rb = (CleanQ_RB_write_head_y b \<acute>RingCRB)   \<rbrace>
-        \<acute>RingCRB :== (CleanQ_RB_incr_head_y b rb) 
-        \<lbrace> CleanQ_RB_Invariants K \<acute> RingCRB \<and> b \<notin> rSY \<acute>RingCRB \<and>
-         enq = CleanQ_RB_enq_x_possible \<acute>RingCRB \<and> CleanQ_RB_deq_x_possible \<acute>RingCRB \<and>
-         deq2 =  CleanQ_RB_deq_y_possible \<acute>RingCRB 
- \<rbrace>"
-  apply(vcg, simp add:CleanQ_RB_enq_y_inv_all CleanQ_RB_enq_y_enq_x_possible)
-  apply (simp add: CleanQ_RB_enq_y_result CleanQ_RB_enq_y_deq_x_possible)
-  by (meson CleanQ_RB_enq_y_deq_y_possible)
+
+paragraph \<open>Y increments the tail pointer\<close>
+
+
+lemma CleanQ_CRB_Dequeue_X_P_incr_tail:
+"\<Gamma>\<turnstile> \<lbrace> CleanQ_RB_deq_x_P K \<acute>RingCRB  \<rbrace> 
+   \<acute>RingCRB :== CleanQ_RB_incr_tail_y by \<acute>RingCRB 
+  \<lbrace> CleanQ_RB_deq_x_P K \<acute>RingCRB   \<rbrace>"
+  apply(vcg, auto)
+  oops
+
+lemma CleanQ_CRB_Dequeue_X_Q_incr_tail:
+"\<Gamma>\<turnstile> \<lbrace> CleanQ_RB_deq_x_Q K \<acute>RingCRB bx  \<rbrace> 
+   \<acute>RingCRB :== CleanQ_RB_incr_tail_y by \<acute>RingCRB   
+  \<lbrace>  CleanQ_RB_deq_x_Q K \<acute>RingCRB bx \<rbrace>"
+  apply(vcg, auto)
+  oops
+
+
+lemma CleanQ_CRB_Dequeue_X_R_incr_tail:
+"\<Gamma>\<turnstile> \<lbrace> CleanQ_RB_deq_x_R K \<acute>RingCRB bx  \<rbrace> 
+   \<acute>RingCRB :== CleanQ_RB_incr_tail_y by \<acute>RingCRB 
+  \<lbrace>  CleanQ_RB_deq_x_R K \<acute>RingCRB bx \<rbrace>"
+  apply(vcg, auto)
+  oops
+
 
 end 
